old/Sample.v
@@ -1,0 +1,25 @@
+Inductive sample : Type :=
+  | nothing : sample
+  | everything : list sample -> sample.
+
+Section Sample.
+
+Variable P : sample → Type.
+Variable Pnothing : P nothing.
+Variable Psomething : ∀ (l : list sample), ilist P l -> P (everything l).
+
+Equations sample_rect' (s : sample) : P s :=
+  sample_rect' nothing := Pnothing;
+  sample_rect' (everything l) := Psomething l (sample_sub_rect' l)
+where sample_sub_rect' (l : list sample) : ilist P l :=
+  sample_sub_rect' [] := tt;
+  sample_sub_rect' (x :: xs) := (sample_rect' x, sample_sub_rect' xs).
+
+End Sample.
+
+Example foo : sample → nat.
+Proof.
+  intros.
+  induction H using sample_rect'.
+  admit.
+
